MathematicalLogic/FirstOrder/Proof/Init.lean
@@ -1,0 +1,20 @@
+import Mathlib.Tactic.Core
+
+namespace FirstOrder.Language.Proof
+
+open Lean Meta
+
+initialize prwExt : SimpleScopedEnvExtension Name (Array Name) ←
+  registerSimpleScopedEnvExtension {
+    addEntry := fun a n => a.push n
+    initial := {}
+  }
+
+initialize registerBuiltinAttribute {
+  name := `prw
+  descr := "generalized congruence"
+  add := fun decl _ kind ↦ MetaM.run' do
+    prwExt.add decl kind
+}
+
+end FirstOrder.Language.Proof
